Proof works, with various holes

theories/embedding.v
@@ -23,6 +23,7 @@ Definition lzero := <lzero>.
 Definition lsuc := <lsuc>.
 Definition pi := <fun x => fun y => fun gamma => Pi (x gamma) (fun a => y (gamma , a))>.
 Definition U : QTerm := <fun lvl => fun env => U lvl>.
+Definition Empty := <fun env => Empty>.
 
 Definition var_to_term := <fun x => x>.
 Definition lambda := <fun t => fun gamma => fun a => t (gamma , a)>.
@@ -43,12 +44,13 @@ Inductive VarTyped : QTerm -> QTerm -> QTerm -> Prop :=
 Inductive Typed : QTerm -> QTerm -> QTerm -> Prop :=
 | ty_lambda : forall ctx A B s, Typed <`cons `ctx `A> B s -> Typed ctx <`pi `A `B> <`lambda `s>
 | ty_app : forall ctx A B s1 s2, Typed ctx <`pi `A `B> s1 -> Typed ctx A s2
-                                 -> Typed ctx <fun env => `B (env , `s2 env)> <`app `s1 `s2>
+                                 -> Typed ctx <fun env => `B [env] (env , (`s2 [env]) env)> <`app `s1 `s2>
 | ty_var : forall ctx T t, VarTyped ctx T t -> Typed ctx T t
 | ty_pi : forall ctx lvl A B,
     Typed ctx <`U `lvl> A
-    -> Typed ctx <`cons ctx A> B -> Typed ctx <`U `lvl> <`pi `A `B>
-| ty_U : forall ctx lvl, Typed ctx <`U `lvl> <`U (`lsuc `lvl)>
+    -> Typed <`cons `ctx `A> <`U `lvl> B -> Typed ctx <`U `lvl> <`pi `A `B>
+| ty_U : forall ctx lvl, Typed ctx <`U (`lsuc `lvl)> <`U `lvl>
+| ty_Empty : forall ctx lvl, Typed ctx <`U `lvl> Empty
 .
 
 Theorem cast {A B : Type} (a : A) (p : A = B) : B.
@@ -72,43 +74,146 @@ Qed.
 Unset Positivity Checking.
 Inductive In : QTerm -> QTerm -> Prop :=
 | in_U : forall lvl, In <U `lvl> <U (`lsuc `lvl)>
-| in_Pi : forall A B f,
-    (forall a, In a A -> In <`f `a> B)
+
+(* Is this right? How should B take a as an input? *)
+| in_fun : forall A B f,
+    (forall a, In a A -> In <`f `a> <`B `a>)
     -> In f <Pi `A `B>
+| in_Pi : forall A B lvl,
+    In A <U `lvl>
+    -> (forall a, In a A -> In <`B `a> <U `lvl>)
+    -> In <Pi `A `B> <U `lvl>
+| in_Empty : forall lvl,
+    In <Empty> <U `lvl>
 .
 (* TODO: should I encode PI as <Pi A B> or <Pi , A , B>?*)
 
 
 Inductive InCtx : QTerm -> QTerm -> Prop :=
-| in_nil : InCtx <nil> <nil>
+| in_nil : InCtx nil nil
 | in_cons : forall env ctx val T,
-    InCtx env ctx -> In val T -> InCtx <`env , `val> <`cons `ctx `T> 
+    InCtx env ctx -> In val <`T `env> -> InCtx <`env , `val> <`cons `ctx `T> 
 .
 
-
+Theorem fundamental_lemma_for_variables : forall ctx T t env,
+    VarTyped ctx T t -> InCtx env ctx -> In <`t `env> <`T `env>.
+Proof.
+  intros.
+  induction H.
+  - inversion H0.
+    + unfold cons in H2.
+      normalize_in H2.
+      (* we need to be able to prove that nil != cons here, but with my representation that doesn' twork*)
+Admitted.      
 
 (* Think about the proof informally first *)
 Theorem fundamental_lemma : forall ctx T t env,
     Typed ctx T t -> InCtx env ctx -> In <`t `env> <`T `env>.
 Proof.
   intros.
+  generalize env, H0.
+  clear H0.
+  clear env.
   induction H.
-  - unfold pi. normalize. repeat fix_subst_lifts.
-    eapply (cast (in_Pi _ _ _ _)). unfold_all.
-    lambda_solve. (* I don't understand what happned to the goal from the arg to in_Pi. How
-                   did it get solved? *)
-  - pose (IHTyped1 H0) as Ih1.
-    pose (IHTyped2 H0) as Ih2.
+  - intros. unfold pi. normalize. repeat fix_subst_lifts.
+    eapply (cast (in_fun _ _ _ _)). unfold_all.
+    lambda_solve.
+    Unshelve. (* This focuses the goal from the argument to in_fun *)
+    intros.
+    normalize. repeat fix_subst_lifts.
+    apply IHTyped.
+    apply in_cons.
+    apply H0.
+    apply H1.
+  - intros.
+    pose (IHTyped1 env H1) as Ih1.
+    pose (IHTyped2 env H1) as Ih2.
     inversion Ih1.
+    (* Prove that it can't be in_U *)
     unfold pi in H4.
     Check eta.
     normalize_in H4.
+    solve_neutral_unequal_case.
+    (* Do the actual real proof for in_fun *)
+    unfold pi in H2.
+    normalize_in H2.
+    repeat fix_subst_lifts_in H2.
+    lambda_solve.
+    repeat neutral_inj_case.
+    lambda_solve.
+    normalize.
+    fix_subst_lifts.
+    apply H4 in Ih2.
+    unfold app.
+    normalize.
+    repeat fix_subst_lifts.
+    
+    apply (cast Ih2).
+    lambda_solve.
+    fix_subst_lifts.
+    reflexivity.
+    (* prove that it can't be in_Pi *)
+    unfold pi in H3.
+    normalize_in H3.
+    solve_neutral_unequal_case.
+    (* prove that it can't be in_Empty *)
+    unfold pi in H4.
+    normalize_in H4.
+    solve_neutral_unequal_case.
+  - intros.
+    apply (fundamental_lemma_for_variables ctx T t env H H0).
+  - intros.
+    unfold pi, U.
+    normalize.
+    repeat fix_subst_lifts.
+    Check in_Pi.
+    apply in_Pi.
+    pose (IHTyped1 env H1) as ih1.
+    unfold U in ih1.
+    normalize_in ih1.
+    fix_subst_lifts_in ih1.
+    apply ih1.
+    intros.
+    normalize.
+    fix_subst_lifts.
+    Check in_cons.
+    pose (IHTyped2 <`env , `a> (in_cons _ _ _ _ H1 H2)) as ih2.
+    unfold U in ih2.
+    normalize_in ih2.
+    fix_subst_lifts_in ih2.
+    apply ih2.
+  - intros.
+    Check in_U.
+    eapply (cast (in_U _)).
+    unfold U.
+    normalize.
+    fix_subst_lifts.
+    lambda_solve.
+  - intros.
+    Check in_Empty.
+    eapply (cast (in_Empty _)).
+    unfold Empty, U.
+    normalize.
+    lambda_solve.
+Qed.
 
-    Check lamInj.
-    match goal with
-    | H : lam ?s ?t1 = lam ?s ?t2 |- _ => apply lamInj in H
-    end.
-    lambda_solve.
-    rewrite (lamInj _ _ "x") in H4.
-    (* we should be able to get a contradiction! *)
-    lambda_solve.
+
+Theorem consistency : forall t,
+    Typed nil Empty t -> False.
+Proof.
+  intros.
+  pose (fundamental_lemma nil Empty t nil H in_nil) as x.
+  inversion x.
+  unfold Empty in H2.
+  normalize_in H2.
+  solve_neutral_unequal_case.
+  unfold Empty in H0.
+  normalize_in H0.
+  solve_neutral_unequal_case.
+  unfold Empty in H1.
+  normalize_in H1.
+  solve_neutral_unequal_case.
+  unfold Empty in H2.
+  normalize_in H2.
+  solve_neutral_unequal_case.
+Qed.
